working on last

Smallstep.v
@@ -767,3 +767,106 @@ Inductive cstep : (com * state) -> (com * state) -> Prop :=
       => (IFB b THEN (c1;; (WHILE b DO c1 END)) ELSE SKIP FI) / st
 
   where " t '/' st '=>' t' '/' st' " := (cstep (t,st) (t',st')).
+
+
+Module CImp.
+
+Inductive com : Type :=
+  | CSkip : com
+  | CAss : id -> aexp -> com
+  | CSeq : com -> com -> com
+  | CIf : bexp -> com -> com -> com
+  | CWhile : bexp -> com -> com
+  (* New: *)
+  | CPar : com -> com -> com.
+
+Notation "'SKIP'" :=
+  CSkip.
+Notation "x '::=' a" :=
+  (CAss x a) (at level 60).
+Notation "c1 ;; c2" :=
+  (CSeq c1 c2) (at level 80, right associativity).
+Notation "'WHILE' b 'DO' c 'END'" :=
+  (CWhile b c) (at level 80, right associativity).
+Notation "'IFB' b 'THEN' c1 'ELSE' c2 'FI'" :=
+  (CIf b c1 c2) (at level 80, right associativity).
+Notation "'PAR' c1 'WITH' c2 'END'" :=
+  (CPar c1 c2) (at level 80, right associativity).
+
+Inductive cstep : (com * state) -> (com * state) -> Prop :=
+    (* Old part *)
+  | CS_AssStep : forall st i a a',
+      a / st =>a a' ->
+      (i ::= a) / st => (i ::= a') / st
+  | CS_Ass : forall st i n,
+      (i ::= (ANum n)) / st => SKIP / (t_update st i n)
+  | CS_SeqStep : forall st c1 c1' st' c2,
+      c1 / st => c1' / st' ->
+      (c1 ;; c2) / st => (c1' ;; c2) / st'
+  | CS_SeqFinish : forall st c2,
+      (SKIP ;; c2) / st => c2 / st
+  | CS_IfTrue : forall st c1 c2,
+      (IFB BTrue THEN c1 ELSE c2 FI) / st => c1 / st
+  | CS_IfFalse : forall st c1 c2,
+      (IFB BFalse THEN c1 ELSE c2 FI) / st => c2 / st
+  | CS_IfStep : forall st b b' c1 c2,
+      b /st =>b b' ->
+          (IFB b THEN c1 ELSE c2 FI) / st 
+      => (IFB b' THEN c1 ELSE c2 FI) / st
+  | CS_While : forall st b c1,
+          (WHILE b DO c1 END) / st 
+      => (IFB b THEN (c1;; (WHILE b DO c1 END)) ELSE SKIP FI) / st
+    (* New part: *)
+  | CS_Par1 : forall st c1 c1' c2 st',
+      c1 / st => c1' / st' ->
+      (PAR c1 WITH c2 END) / st => (PAR c1' WITH c2 END) / st'
+  | CS_Par2 : forall st c1 c2 c2' st',
+      c2 / st => c2' / st' ->
+      (PAR c1 WITH c2 END) / st => (PAR c1 WITH c2' END) / st'
+  | CS_ParDone : forall st,
+      (PAR SKIP WITH SKIP END) / st => SKIP / st
+  where " t '/' st '=>' t' '/' st' " := (cstep (t,st) (t',st')).
+
+Definition cmultistep := multi cstep.
+
+Notation " t '/' st '=>*' t' '/' st' " :=
+   (multi cstep (t,st) (t',st'))
+   (at level 40, st at level 39, t' at level 39).
+
+Definition par_loop : com :=
+  PAR
+    Y ::= ANum 1
+  WITH
+    WHILE BEq (AId Y) (ANum 0) DO
+      X ::= APlus (AId X) (ANum 1)
+    END
+  END.
+
+Example par_loop_example_0:
+  exists st',
+       par_loop / empty_state =>* SKIP / st'
+    /\ st' X = 0.
+Proof.
+  eapply ex_intro. split.
+  unfold par_loop.
+  eapply multi_step. apply CS_Par1.
+    apply CS_Ass.
+  eapply multi_step. apply CS_Par2. apply CS_While.
+  eapply multi_step. apply CS_Par2. apply CS_IfStep.
+    apply BS_Eq1. apply AS_Id.
+  eapply multi_step. apply CS_Par2. apply CS_IfStep.
+    apply BS_Eq. simpl.
+  eapply multi_step. apply CS_Par2. apply CS_IfFalse.
+  eapply multi_step. apply CS_ParDone.
+  eapply multi_refl.
+  reflexivity. Qed.
+
+
+Lemma par_body_n__Sn : forall n st,
+  st X = n /\ st Y = 0 ->
+  par_loop / st =>* par_loop / (t_update st X (S n)).
+Proof.
+  intros. eapply multi_step. apply CS_Par2. apply CS_While.
+  eapply multi_step. apply CS_Par2. apply CS_IfStep.
+    apply BS_Eq1. apply AS_Id.
+  
